Complete explanation and skeleton file for IntTree.

src/dafny/smart/IntTree.dfy
@@ -12,11 +12,13 @@
  * under the License.
  */
 
+include "Helpers.dfy"
 include "Trees.dfy"
 include "MerkleTrees.dfy"
 
 module DiffTree {
 
+    import opened Helpers
     import opened Trees
     import opened MerkleTrees
 
@@ -52,23 +54,117 @@ module DiffTree {
 
     /**
      *  Incremental algorithm.
+     *
+     *  @todo   Add data structures and complete method add to
+     *          correctly compute diffRoot. 
      */
     class IntTree {
 
-        constructor()
+        /**  The root tracking the Merkle Tree. */
+        ghost var root : Node<int>
 
-        method incrDiffAlgo(root: Node<int>, l: seq<int>, e: int) returns (root' : Node<int>) 
-            requires isCompleteTree(root)
-            requires |l| < |collectLeaves(root)|
-            requires MerkleTrees.treeLeftmostLeavesMatchList(l, root, 0)
+        /** Height if the tree */
+        var height : nat 
 
-            ensures isCompleteTree(root')
-            ensures height(root') == height(root)
-            ensures MerkleTrees.treeLeftmostLeavesMatchList(l + [e], root', 0)
+        /** diffRoot, the value of diff on the root. */
+        var diffRoot : int
+
+        /** Number of elements in the tree. */
+        // var counter : nat
+
+        ghost var store : seq<int>
+
+        /** A valid configuration. */
+        predicate isValid() 
+            requires Trees.isCompleteTree(root)
+            reads this
         {
+            completeTreeNumberOfLeaves(root);
 
+            //  tree correctly decorated by diff.
+            isDecoratedWithDiff(root)
+            //  diffRoot is the value of diff on root.
+            && diffRoot == root.v
+            //  height preserved.
+            && height == Trees.height(root) 
+            && 0 <= |store| <= power2(height - 1)
+            && |collectLeaves(root)| == power2(height - 1)
+
+            //  tree leftmost leaves are in store.
+            && MerkleTrees.treeLeftmostLeavesMatchList(store, root, 0)
+        }
+
+        /**
+         *  Initial tree of height h and all leaves set to 0.
+         */
+        constructor(h: nat) 
+            requires h >= 1
+            ensures Trees.height(root) == h == height
+            ensures MerkleTrees.treeLeftmostLeavesMatchList([], root, 0)
+            ensures store == []
+            ensures Trees.isCompleteTree(root)
+            ensures isValid()
+
+        /** Defines the Int Tree for a given sequence.
+         *  
+         *  @note   This function does not compute the tree but rather
+         *          defines its properties: correctly stores the attribute
+         *          `diff` and the leftmost |l| leaves store l.
+         */
+        function buildMerkle(l: seq<int>, h : nat) : Node<int> 
+            requires h >= 1
+            requires |l| <= power2(h - 1)
+            ensures Trees.height(buildMerkle(l, h)) == h
+            ensures Trees.isCompleteTree(buildMerkle(l, h))
+            ensures |collectLeaves(buildMerkle(l, h))| == power2(h - 1)
+            ensures isDecoratedWithDiff(buildMerkle(l, h))
+            ensures treeLeftmostLeavesMatchList(l, buildMerkle(l, h), 0)
+
+        /** 
+         *  Add element e to the tree.
+         *
+         *  @param  e   The element to add to the store.
+         *
+         *  @todo       This algorithm should maintain the invariant
+         *              `diffRoot == root.v`.
+         */
+        method add(e: int)
+            //  Store is not full
+
+            requires Trees.isCompleteTree(root)
+            requires isValid()
+            requires |store| < power2(height - 1)
+
+            //  Preserves tree height and completeness
+            ensures height == old(height) == Trees.height(root) 
+            ensures Trees.isCompleteTree(root)
+
+            //  Store is updated
+            ensures store == old(store) + [ e ]
+
+            ensures |collectLeaves(root)| == power2(height - 1)
+
+            //  diffRoot stores value of diff for store
+            ensures isDecoratedWithDiff(root)
+            ensures |store| <= power2(height - 1)
+            ensures MerkleTrees.treeLeftmostLeavesMatchList(store, root, 0)
+
+            //  The next one is not verified in the current version of this algo.
+            ensures diffRoot == root.v
+
+            // ensures isValid()
+
+            modifies this
+        {
+            //  Update store
+            store := store + [ e ] ;
+            
+            //  Define new tree for updated store
+            root := buildMerkle(store, height);
+
+            //  Compute the new diffRoot
+            diffRoot := 0 ;
         }
 
     } 
-
 }
